Tidying things up

BSWLean/CNF.lean
@@ -41,24 +41,11 @@ abbrev Clause (vars : Variables) := Finset (Literal vars)
 def Clause.variables {vars} (c : Clause vars) : Finset Variable :=
   c.image Literal.variable
 
-@[simp]
-lemma literal_in_clause_variables {vars} (l : Literal vars) (c : Clause vars)
-: l ∈ c → l.variable ∈ c.variables := by
-  intro h_l_in_c
+@[aesop unsafe]
+lemma literal_in_clause_variables {vars} {l : Literal vars} {c : Clause vars} (h_l_in_c : l ∈ c) :
+    l.variable ∈ c.variables := by
   unfold Clause.variables
   exact Finset.mem_image_of_mem Literal.variable h_l_in_c
-
-@[simp]
-lemma variable_in_clause_variables_implies_literal_in_clause {vars} (v : Variable) (c : Clause vars)
-    (h_v_mem_vars : v ∈ vars) (h_v_mem_c : (v.toLiteral h_v_mem_vars ∈ c) ∨
-                                           (v.toNegLiteral h_v_mem_vars ∈ c))
-    : v ∈ c.variables := by
-  unfold Clause.variables
-  cases h_v_mem_c
-  case inl h_lit_pos_in_c =>
-    exact Finset.mem_image_of_mem Literal.variable h_lit_pos_in_c
-  case inr h_lit_neg_in_c =>
-    exact Finset.mem_image_of_mem Literal.variable h_lit_neg_in_c
 
 abbrev CNFFormula (vars : Variables) := Finset (Clause vars)
 
@@ -73,28 +60,24 @@ def Literal.negate {vars} (l : Literal vars) : (Literal vars) :=
   | .neg v h_v_mem_vars => Literal.pos v h_v_mem_vars
 
 @[simp]
-lemma Literal.eval_negate_eq_not_eval {vars} (l : Literal vars) (a : Assignment vars)
-: l.negate.eval a = ¬ l.eval a := by
-  unfold Literal.eval
-  unfold Literal.negate
+lemma Literal.eval_negate_eq_not_eval {vars} (l : Literal vars) (a : Assignment vars) :
+    l.negate.eval a = ¬ l.eval a := by
+  unfold Literal.eval Literal.negate
   simp only [Bool.not_eq_true, eq_iff_iff, Bool.coe_true_iff_false]
   cases l
   case pos v h_v_mem_vars =>
     rfl
   case neg v h_v_mem_vars =>
-    simp only [Bool.not_not]
+    simp
 
 @[simp]
-lemma Literal.neg_polarity {vars} (l : Literal vars)
-: l.negate.polarity = ¬l.polarity := by
-  unfold polarity
-  unfold negate
+lemma Literal.neg_polarity {vars} (l : Literal vars) : l.negate.polarity = ¬l.polarity := by
+  unfold polarity negate
 
   aesop
 
 @[simp]
-lemma Literal.neg_neg {vars} (l : Literal vars)
-: l.negate.negate = l := by
+lemma Literal.neg_neg {vars} (l : Literal vars) : l.negate.negate = l := by
   unfold negate
 
   aesop
@@ -107,121 +90,108 @@ def CNFFormula.eval {vars} (φ : CNFFormula vars) (a : Assignment vars) : Bool :
 
 
 lemma CNFFormula.eval_eq_false_iff_exists_falsified_clause {vars} (φ : CNFFormula vars)
-    (a : Assignment vars)
-: φ.eval a = false ↔ (∃ c, c ∈ φ ∧ c.eval a = false) := by
+    (a : Assignment vars) : φ.eval a = false ↔ (∃ c, c ∈ φ ∧ c.eval a = false) := by
   constructor
+
   case mpr =>
     intro h_exists_falsified_clause
     unfold CNFFormula.eval
     obtain ⟨c, h_c_in_φ, h_c_eval_a_false⟩ := h_exists_falsified_clause
     let φ' := φ.erase c
+
     have h_c_not_in_φ' : c ∉ φ' := by
       rw [Finset.mem_erase]
-      simp only [ne_eq, not_true_eq_false, false_and, not_false_eq_true]
+      simp
+
     have : φ = insert c φ' := by
       rw [Finset.insert_erase h_c_in_φ]
+
     rw [this]
     rw [Finset.fold_insert h_c_not_in_φ']
     rw [h_c_eval_a_false]
     rfl
+
   case mp =>
     intro h_φ_eval_a_false
     contrapose! h_φ_eval_a_false
     simp only [ne_eq, Bool.not_eq_false]
-    simp only [ne_eq, Bool.not_eq_false] at h_φ_eval_a_false
-    rename ∀ c ∈ φ, c.eval a = true => h_all_sat
     unfold CNFFormula.eval
     induction φ using Finset.induction_on with
     | empty =>
       trivial
     | insert c φ' h_c_not_in_φ' ih =>
-      rw [Finset.fold_insert h_c_not_in_φ']
-      rw [ih]
-
-      · simp only [Bool.and_true]
-        apply h_all_sat
-        exact Finset.mem_insert_self c φ'
-      · intro c' h_c'_in_φ'
-        apply h_all_sat
-        exact Finset.mem_insert_of_mem h_c'_in_φ'
+      aesop
 
 lemma Clause.eval_eq_true_iff_exists_satisfied_literal {vars} (c : Clause vars)
-    (a : Assignment vars)
-: c.eval a = true ↔ (∃ l, l ∈ c ∧ l.eval a = true) := by
+    (a : Assignment vars) : c.eval a = true ↔ (∃ l, l ∈ c ∧ l.eval a = true) := by
   constructor
+
   case mpr =>
     intro h_exists_falsified_c
     unfold Clause.eval
     obtain ⟨l, h_l_in_c, h_l_eval_a_false⟩ := h_exists_falsified_c
     let c' := c.erase l
+
     have h_l_not_in_c' : l ∉ c' := by
       rw [Finset.mem_erase]
-      simp only [ne_eq, not_true_eq_false, false_and, not_false_eq_true]
+      simp
+
     have : c = insert l c' := by
       rw [Finset.insert_erase h_l_in_c]
+
     rw [this]
     rw [Finset.fold_insert h_l_not_in_c']
     rw [h_l_eval_a_false]
     rfl
+
   case mp =>
     intro h_c_eval_a_false
     contrapose! h_c_eval_a_false
     simp only [ne_eq, Bool.not_eq_true]
     simp only [ne_eq, Bool.not_eq_true] at h_c_eval_a_false
-    rename ∀ l ∈ c, l.eval a = false => h_all_unsat
     unfold Clause.eval
     induction c using Finset.induction_on with
     | empty =>
       trivial
     | insert l c' h_l_not_in_c' ih =>
-      rw [Finset.fold_insert h_l_not_in_c']
-      rw [ih]
+      aesop
 
-      · simp only [Bool.or_false]
-        apply h_all_unsat
-        exact Finset.mem_insert_self l c'
-      · intro l' h_l'_in_c'
-        apply h_all_unsat
-        exact Finset.mem_insert_of_mem h_l'_in_c'
-
-lemma neg_iff (A : Prop) (B : Prop) : (A ↔ B) ↔ (¬A ↔ ¬B) := by tauto
+lemma neg_iff (A : Prop) (B : Prop) : (¬A ↔ ¬B) ↔ (A ↔ B) := by tauto
 
 lemma CNFFormula.eval_eq_true_iff_all_satisfied_clauses {vars} (φ : CNFFormula vars)
-    (a : Assignment vars)
-: φ.eval a = true ↔ (∀ c, c ∈ φ → c.eval a = true) := by
-  rw [neg_iff]
+    (a : Assignment vars) : φ.eval a = true ↔ (∀ c, c ∈ φ → c.eval a = true) := by
+  rw [←neg_iff]
   push_neg
   simp only [ne_eq, Bool.not_eq_true]
   exact eval_eq_false_iff_exists_falsified_clause φ a
 
 lemma Clause.eval_eq_false_iff_all_falsified_literals {vars} (c : Clause vars)
-    (a : Assignment vars)
-: c.eval a = false ↔ (∀ l, l ∈ c → l.eval a = false) := by
-  rw [neg_iff]
+    (a : Assignment vars) : c.eval a = false ↔ (∀ l, l ∈ c → l.eval a = false) := by
+  rw [←neg_iff]
   push_neg
   simp only [ne_eq, Bool.not_eq_false]
   exact eval_eq_true_iff_exists_satisfied_literal c a
 
-def Clause.resolve {vars} (c₁ : Clause vars) (c₂ : Clause vars) (x : Variable) (h_x : x ∈ vars)
-: Clause vars :=
+def Clause.resolve {vars} (c₁ c₂ : Clause vars) (x : Variable) (h_x : x ∈ vars) :
+    Clause vars :=
   c₁.erase (x.toLiteral h_x) ∪ c₂.erase (x.toNegLiteral h_x)
 
-@[simp]
-lemma Clause.not_in_variables_subset {vars} (c₁ : Clause vars) (c₂ : Clause vars) (x : Variable) :
-    c₁ ⊆ c₂ → x ∉ c₂.variables → x ∉ c₁.variables := by
-  intro h_subset
+@[aesop unsafe]
+lemma Clause.not_in_variables_subset {vars} {c₁ c₂ : Clause vars} {x : Variable}
+    (h_subset : c₁ ⊆ c₂) (h : x ∉ c₂.variables) : x ∉ c₁.variables := by
   unfold Clause.variables
+  unfold Clause.variables at h
   aesop
 
 @[simp]
-lemma Clause.union_variables {vars} (c₁ : Clause vars) (c₂ : Clause vars) :
+lemma Clause.union_variables {vars} (c₁ c₂ : Clause vars) :
     (c₁ ∪ c₂).variables = c₁.variables ∪ c₂.variables := by
   unfold Clause.variables
   aesop
 
-lemma Clause.subset_variables {vars} (c₁ : Clause vars) (c₂ : Clause vars) :
-    c₁ ⊆ c₂ → c₁.variables ⊆ c₂.variables := by
-  intro h
+@[aesop unsafe]
+lemma Clause.subset_variables {vars} {c₁ c₂ : Clause vars} (h : c₁ ⊆ c₂) :
+    c₁.variables ⊆ c₂.variables := by
   unfold Clause.variables
   rw [@Finset.image_subset_iff]
   intro l h_l
