BSWLean/Conversion.lean
@@ -9,40 +9,36 @@ def Assignment.negVariable {vars} (ρ : Assignment vars) (v : Variable) : Option
   else
     none
 
-@[simp]
-lemma Assignment.negVariable_variable {vars} (ρ : Assignment vars)
-    (v : Variable) : ∀ y ∈ Assignment.negVariable ρ v, y.variable = v := by
-  intro y h
+@[aesop unsafe]
+lemma Assignment.negVariable_variable {vars} {ρ : Assignment vars} {v : Variable}
+    {y : Literal vars} (h : y ∈ Assignment.negVariable ρ v) : y.variable = v := by
   unfold Assignment.negVariable at h
-
   aesop
 
 
 @[simp]
-lemma Assignment.negVariable_inj {vars} (ρ : Assignment vars) :
-  ∀ (x₁ x₂ : Variable), ∀ y ∈ Assignment.negVariable ρ x₁,
-    y ∈ Assignment.negVariable ρ x₂ → x₁ = x₂ := by
-  intros x₁ x₂ y h_y_in_mp_x1 h_y_in_mp_x2
+lemma Assignment.negVariable_inj {vars} {ρ : Assignment vars} {x₁ x₂ : Variable} {y : Literal vars}
+    (h_y_in_mp_x1 : y ∈ ρ.negVariable x₁) (h_y_in_mp_x2 : y ∈ ρ.negVariable x₂) : x₁ = x₂ := by
   unfold Assignment.negVariable at h_y_in_mp_x1 h_y_in_mp_x2
   simp_all only [Option.mem_def, Option.dite_none_right_eq_some]
   obtain ⟨h_x1_in_vars, h_y_eq_lit1⟩ := h_y_in_mp_x1
   obtain ⟨h_x2_in_vars, h_y_eq_lit2⟩ := h_y_in_mp_x2
-  unfold Variable.toLiteral at h_y_eq_lit1 h_y_eq_lit2
-  unfold Variable.toNegLiteral at h_y_eq_lit1 h_y_eq_lit2
-
+  unfold Variable.toLiteral Variable.toNegLiteral at h_y_eq_lit1 h_y_eq_lit2
   aesop
 
-lemma Assignment.negVariable_some_iff_variable_in_vars {vars} (ρ : Assignment vars) (v : Variable) :
-  (Assignment.negVariable ρ v).isSome ↔ v ∈ vars := by
+@[simp]
+lemma Assignment.negVariable_some_iff_variable_in_vars {vars} {ρ : Assignment vars} {v} :
+    (ρ.negVariable v).isSome ↔ v ∈ vars := by
   unfold Assignment.negVariable
 
   aesop
 
 def Assignment.toClause {vars} (ρ : Assignment vars) : Clause vars :=
-  vars.filterMap (Assignment.negVariable ρ) (Assignment.negVariable_inj ρ)
+  vars.filterMap (ρ.negVariable) (by exact fun a a' b a_1 a_2 ↦ negVariable_inj a_1 a_2)
 
+@[simp]
 lemma Assignment.in_toClause {vars} (ρ : Assignment vars) (l : Literal vars) :
-  l ∈ ρ.toClause ↔ (l.variable ∈ vars ∧ l.eval ρ = false) := by
+    l ∈ ρ.toClause ↔ (l.variable ∈ vars ∧ l.eval ρ = false) := by
   unfold Assignment.toClause
   simp only [Finset.mem_filterMap, Literal.variable_mem_vars, true_and]
   constructor
@@ -50,42 +46,18 @@ lemma Assignment.in_toClause {vars} (ρ : Assignment vars) (l : Literal vars) :
     intro h_l_in_toClause
     use l.variable
     simp only [Literal.variable_mem_vars, true_and]
-    unfold Assignment.negVariable
-    unfold Literal.variable
+    unfold Assignment.negVariable Literal.variable
     unfold Literal.eval at h_l_in_toClause
-    simp_all only [Option.dite_none_right_eq_some]
-    split
-    next l v
-      h_v_mem_vars =>
-      simp_all only [Bool.false_eq_true, ↓reduceIte, Option.some.injEq, exists_true_left]
-      rfl
-    next l v
-      h_v_mem_vars =>
-      simp_all only [Bool.not_eq_eq_eq_not, Bool.not_false, ↓reduceIte, Option.some.injEq,
-                     exists_true_left]
-      rfl
+    aesop
   case mp =>
     intro h
     obtain ⟨v, ⟨h_v_in_vars, h_l_eval_ρ_false⟩⟩ := h
-    unfold Assignment.negVariable at h_l_eval_ρ_false
+    unfold Assignment.negVariable Variable.toLiteral Variable.toNegLiteral at h_l_eval_ρ_false
     unfold Literal.eval
-    unfold Variable.toLiteral Variable.toNegLiteral at h_l_eval_ρ_false
+    aesop
 
-    simp_all only [↓reduceDIte]
-    split
-    next l v_1 h_v_mem_vars =>
-      split at h_l_eval_ρ_false
-      next h => simp_all only [Option.some.injEq, reduceCtorEq]
-      next h => simp_all only [Bool.not_eq_true, Option.some.injEq, Literal.pos.injEq]
-    next l v_1 h_v_mem_vars =>
-      simp_all only [Bool.not_eq_eq_eq_not, Bool.not_false]
-      split at h_l_eval_ρ_false
-      next h => simp_all only [Option.some.injEq, Literal.neg.injEq]
-      next h => simp_all only [Bool.not_eq_true, Option.some.injEq, reduceCtorEq]
-
-
-lemma Assignment.toClause_eval {vars} (ρ : Assignment vars) :
-  ρ.toClause.eval ρ = false := by
+@[simp]
+lemma Assignment.toClause_eval {vars} (ρ : Assignment vars) : ρ.toClause.eval ρ = false := by
   unfold Assignment.toClause
   rw [Clause.eval_eq_false_iff_all_falsified_literals]
   intro l
@@ -98,8 +70,8 @@ lemma Assignment.toClause_eval {vars} (ρ : Assignment vars) :
 
   aesop
 
-lemma Assignment.toClause_variables {vars} (ρ : Assignment vars) :
-  ρ.toClause.variables = vars := by
+@[simp]
+lemma Assignment.toClause_variables {vars} (ρ : Assignment vars) : ρ.toClause.variables = vars := by
   unfold Clause.variables
   ext v
   constructor
@@ -120,23 +92,14 @@ lemma Assignment.toClause_variables {vars} (ρ : Assignment vars) :
       simp_all only [↓reduceDIte]
       split
       next h =>
-        simp_all only [Option.get_some]
-        unfold Variable.toNegLiteral
-        unfold Literal.eval
-        simp_all only [Bool.not_true]
+        unfold Variable.toNegLiteral Literal.eval
+        aesop
       next h =>
-        simp_all only [Option.get_some]
-        simp_all only [Bool.not_eq_true]
-        exact h
+        aesop
 
     · unfold l_some l
-      rw [negVariable_variable ρ]
-      simp only [Option.mem_def, Option.some_get]
+      aesop
 
   case mp =>
     intro a
-    simp_all only [Finset.mem_image]
-    obtain ⟨w, h⟩ := a
-    obtain ⟨left, right⟩ := h
-    subst right
-    simp_all only [Literal.variable_mem_vars]
+    aesop
