BSWLean/Substitutions.lean
@@ -1,22 +1,19 @@
 import BSWLean.CNF
 
-def Literal.restrict {vars} (l : Literal vars)
-    (sub_vars : Variables) (h_mem : l.variable ∈ sub_vars)
-    : Literal sub_vars :=
+def Literal.restrict {vars} (l : Literal vars) (sub_vars : Variables)
+    (h_mem : l.variable ∈ sub_vars) : Literal sub_vars :=
   match l with
   | .pos v _ => Literal.pos v h_mem
   | .neg v _ => Literal.neg v h_mem
 
-lemma Literal.restrict_inj {vars} (l₁ : Literal vars) (l₂ : Literal vars)
-  (sub_vars : Variables) (h_l₁_mem : l₁.variable ∈ sub_vars) (h_l₂_mem : l₂.variable ∈ sub_vars)
-  : l₁.restrict sub_vars h_l₁_mem = l₂.restrict sub_vars h_l₂_mem → l₁ = l₂ := by
-  intros h_eq
+lemma Literal.restrict_inj {vars sub_vars} {l₁ l₂ : Literal vars}
+    (h_l₁_mem : l₁.variable ∈ sub_vars) (h_l₂_mem : l₂.variable ∈ sub_vars)
+    (h_eq : l₁.restrict sub_vars h_l₁_mem = l₂.restrict sub_vars h_l₂_mem) : l₁ = l₂ := by
   unfold Literal.restrict at h_eq
   cases l₁ <;> cases l₂ <;> simp_all
 
-def Clause.shrink {vars} (c : Clause vars)
-    (keep_vars : Variables) (h_mem : ∀ l, l ∈ c → l.variable ∈ keep_vars)
-    : Clause keep_vars :=
+def Clause.shrink {vars} (c : Clause vars) (keep_vars : Variables)
+    (h_mem : ∀ l, l ∈ c → l.variable ∈ keep_vars) : Clause keep_vars :=
   let f := fun l : Literal vars =>
       if h : l ∈ c then some (l.restrict keep_vars (h_mem l h)) else none
 
@@ -27,20 +24,15 @@ def Clause.shrink {vars} (c : Clause vars)
     obtain ⟨_, h⟩ := h₁
     obtain ⟨h_l₂_c, h_l₂_b⟩ := h₂
     rw [←h_l₂_b] at h
-    have h_l₁_vars : l₁.variable ∈ keep_vars := by (expose_names; exact h_mem l₁ w)
-    have h_l₂_vars : l₂.variable ∈ keep_vars := by (expose_names; exact h_mem l₂ h_l₂_c)
+    have h_l₁_vars : l₁.variable ∈ keep_vars := by simp_all
+    have h_l₂_vars : l₂.variable ∈ keep_vars := by simp_all
     unfold Literal.restrict at h
-    expose_names;
-    exact
-      Literal.restrict_inj l₁ l₂ keep_vars
-        (h_mem l₁ ((Iff.of_eq (Eq.refl (l₁ ∈ c))).mpr w))
-        (h_mem l₂ ((Iff.of_eq (Eq.refl (l₂ ∈ c))).mpr h_l₂_c)) h
+    aesop
 
   c.filterMap f this
 
-def Clause.split {vars} (c : Clause vars)
-    (split_vars : Variables)
-    : (Clause (vars ∩ split_vars)) × (Clause (vars \ split_vars)) :=
+def Clause.split {vars} (c : Clause vars) (split_vars : Variables) :
+    (Clause (vars ∩ split_vars)) × (Clause (vars \ split_vars)) :=
   let c_in := c.filter (fun l => l.variable ∈ split_vars)
   let c_out := c.filter (fun l => l.variable ∉ split_vars)
 
@@ -50,7 +42,7 @@ def Clause.split {vars} (c : Clause vars)
     simp only [Finset.mem_filter] at h_c_in
     rw [@Finset.mem_inter]
     constructor
-    · simp only [Literal.variable_mem_vars]
+    · simp
     · apply h_c_in.2
 
   have h_out : ∀ l, l ∈ c_out → l.variable ∈ (vars \ split_vars) := by
@@ -59,46 +51,37 @@ def Clause.split {vars} (c : Clause vars)
     simp only [Finset.mem_filter] at h_c_out
     simp only [Finset.mem_sdiff]
     constructor
-    · simp only [Literal.variable_mem_vars]
+    · simp
     · apply h_c_out.2
-
 
   let c_in' := Clause.shrink c_in (vars ∩ split_vars) h_in
   let c_out' := Clause.shrink c_out (vars \ split_vars) h_out
 
   (c_in', c_out')
 
-def Assignment.restrict {vars} (ρ : Assignment vars)
-    (sub_vars : Variables) (h_subset : sub_vars ⊆ vars) : Assignment sub_vars :=
+def Assignment.restrict {vars} (ρ : Assignment vars) (sub_vars : Variables)
+    (h_subset : sub_vars ⊆ vars) : Assignment sub_vars :=
   have : ∀ v ∈ sub_vars, v ∈ vars := by
     exact fun v a ↦ h_subset a
 
   fun v h_v_mem_sub_vars => ρ v (this v h_v_mem_sub_vars)
 
 @[simp]
-lemma Assignment.double_restrict {vars} (ρ : Assignment vars)
-    (sub_vars₁ : Variables) (h_subset₁ : sub_vars₁ ⊆ vars)
-    (sub_vars₂ : Variables) (h_subset₂ : sub_vars₂ ⊆ sub_vars₁)
-  : (ρ.restrict sub_vars₁ h_subset₁).restrict sub_vars₂ h_subset₂ =
+lemma Assignment.double_restrict {vars sub_vars₁ sub_vars₂} (ρ : Assignment vars)
+    (h_subset₁ : sub_vars₁ ⊆ vars) (h_subset₂ : sub_vars₂ ⊆ sub_vars₁) :
+    (ρ.restrict sub_vars₁ h_subset₁).restrict sub_vars₂ h_subset₂ =
     ρ.restrict sub_vars₂ (by exact fun ⦃a⦄ a_1 ↦ h_subset₁ (h_subset₂ a_1)) := by
   rfl
 
-lemma Literal.restrict_correctness {vars} (l : Literal vars) (sub_vars : Variables)
-  (ρ : Assignment vars) (h_subset : sub_vars ⊆ vars) (h_l : l.variable ∈ sub_vars)
-  : l.eval ρ = (l.restrict sub_vars h_l).eval (ρ.restrict sub_vars h_subset) := by
+@[simp]
+lemma Literal.restrict_correctness {vars sub_vars} {l : Literal vars} {ρ : Assignment vars}
+    (h_subset : sub_vars ⊆ vars) (h_l : l.variable ∈ sub_vars) :
+    (l.restrict sub_vars h_l).eval (ρ.restrict sub_vars h_subset) = l.eval ρ := by
   unfold Literal.restrict
-  unfold Literal.eval
-  unfold Assignment.restrict
-  cases l
-  case pos v h_v_mem_vars =>
-    simp only
-  case neg v h_v_mem_vars =>
-    simp only
+  aesop
 
-
-def Clause.substitute {vars} (c : Clause vars)
-    {sub_vars : Variables} (ρ : Assignment sub_vars)
-    : Option (Clause (vars \ sub_vars)) :=
+def Clause.substitute {vars sub_vars} (c : Clause vars) (ρ : Assignment sub_vars) :
+    Option (Clause (vars \ sub_vars)) :=
   let (c_in, c_out) := Clause.split c sub_vars
 
   if c_in.eval (ρ.restrict (vars ∩ sub_vars) Finset.inter_subset_right) then
@@ -106,34 +89,28 @@ def Clause.substitute {vars} (c : Clause vars)
   else
     some c_out
 
-lemma Clause.substitute_eq_none_iff_eval_subclause_true {vars} (c : Clause vars)
-    (sub_vars : Variables) (ρ : Assignment sub_vars)
-: c.substitute ρ = none ↔
-  (c.split sub_vars).1.eval (ρ.restrict (vars ∩ sub_vars) Finset.inter_subset_right) := by
+lemma Clause.substitute_eq_none_iff_eval_subclause_true {vars sub_vars} (c : Clause vars)
+    (ρ : Assignment sub_vars) :
+    c.substitute ρ = none ↔
+    (c.split sub_vars).1.eval (ρ.restrict (vars ∩ sub_vars) Finset.inter_subset_right) := by
   unfold Clause.substitute
-  constructor
-  case mp =>
-    simp_all only [ite_eq_left_iff, Bool.not_eq_true, reduceCtorEq, imp_false, Bool.not_eq_false,
-      implies_true]
-  case mpr =>
-    simp_all only [↓reduceIte, implies_true]
+  aesop
 
-lemma Clause.substitute_isSome_iff_eval_subclause_false {vars} (c : Clause vars)
-    (sub_vars : Variables) (ρ : Assignment sub_vars)
-: (c.substitute ρ).isSome ↔
-  ¬(c.split sub_vars).1.eval (ρ.restrict (vars ∩ sub_vars) Finset.inter_subset_right) := by
+lemma Clause.substitute_isSome_iff_eval_subclause_false {vars sub_vars} (c : Clause vars)
+    (ρ : Assignment sub_vars) :
+    (c.substitute ρ).isSome ↔
+    ¬(c.split sub_vars).1.eval (ρ.restrict (vars ∩ sub_vars) Finset.inter_subset_right) := by
   rw [← @substitute_eq_none_iff_eval_subclause_true]
   exact Option.isSome_iff_ne_none
 
 @[simp]
-lemma Assignment.restrict_correctness {vars} {h} (ρ : Assignment vars)
-    : ρ.restrict vars h = ρ := by
+lemma Assignment.restrict_correctness {vars} {h} (ρ : Assignment vars) : ρ.restrict vars h = ρ := by
   rfl
 
-lemma Clause.split_correctness {vars} (c : Clause vars)
-    (sub_vars : Variables) (ρ : Assignment vars) (h₁) (h₂) :
-    c.eval ρ = ((c.split sub_vars).1.eval (ρ.restrict (vars ∩ sub_vars) h₁)
-            || (c.split sub_vars).2.eval (ρ.restrict (vars \ sub_vars) h₂)) := by
+lemma Clause.split_correctness {vars} (c : Clause vars) (sub_vars : Variables)
+    (ρ : Assignment vars) :
+    c.eval ρ = ((c.split sub_vars).1.eval (ρ.restrict (vars ∩ sub_vars) (by aesop)) ||
+                (c.split sub_vars).2.eval (ρ.restrict (vars \ sub_vars) (by aesop))) := by
   by_cases h_c : c.eval ρ
 
   case pos =>
@@ -145,49 +122,27 @@ lemma Clause.split_correctness {vars} (c : Clause vars)
     case pos =>
       left
       rw [Clause.eval_eq_true_iff_exists_satisfied_literal]
-      let l' := l.restrict (vars ∩ sub_vars) (by
-        simp only [Finset.mem_inter, Literal.variable_mem_vars, true_and]
-        exact h_l_in_c_in
-      )
-      have h_unfold : l' = l.restrict (vars ∩ sub_vars) (by
-        simp only [Finset.mem_inter, Literal.variable_mem_vars, true_and]
-        exact h_l_in_c_in
-      ) := by
-        rfl
+      let l' := l.restrict (vars ∩ sub_vars) (by aesop)
       have h_l'_in_c_in : l' ∈ (c.split sub_vars).1 := by
-        unfold Clause.split
-        simp only
-        unfold Clause.shrink
+        unfold Clause.split Clause.shrink
         simp only [Finset.mem_filter, Finset.mem_filterMap, Option.dite_none_right_eq_some,
           Option.some.injEq, and_exists_self]
         use l
-        have : l ∈ c ∧ l.variable ∈ sub_vars := by
-          constructor
-          · assumption
-          · assumption
+        have : l ∈ c ∧ l.variable ∈ sub_vars := by aesop
         use this
-      have h_l'_eval : l'.eval (ρ.restrict (vars ∩ sub_vars) h₁) := by
-        rw [h_unfold]
-        rw [←Literal.restrict_correctness l (vars ∩ sub_vars) ρ]
-        assumption
+      have h_l'_eval : l'.eval (ρ.restrict (vars ∩ sub_vars) (by aesop)) := by
+        unfold l'
+        aesop
 
       use l'
     case neg =>
       right
       rw [Clause.eval_eq_true_iff_exists_satisfied_literal]
-      let l' := l.restrict (vars \ sub_vars) (by
-        simp only [Finset.mem_sdiff, Literal.variable_mem_vars, true_and]
-        exact h_l_in_c_in
-      )
-      have h_unfold : l' = l.restrict (vars \ sub_vars) (by
-        simp only [Finset.mem_sdiff, Literal.variable_mem_vars, true_and]
-        exact h_l_in_c_in
-      ) := by
+      let l' := l.restrict (vars \ sub_vars) (by aesop)
+      have h_unfold : l' = l.restrict (vars \ sub_vars) (by aesop) := by
         rfl
       have h_l'_in_c_in : l' ∈ (c.split sub_vars).2 := by
-        unfold Clause.split
-        simp only
-        unfold Clause.shrink
+        unfold Clause.split Clause.shrink
         simp only [Finset.mem_filter, Finset.mem_filterMap, Option.dite_none_right_eq_some,
           Option.some.injEq, and_exists_self]
         use l
@@ -196,10 +151,9 @@ lemma Clause.split_correctness {vars} (c : Clause vars)
           · assumption
           · assumption
         use this
-      have h_l'_eval : l'.eval (ρ.restrict (vars \ sub_vars) h₂) := by
+      have h_l'_eval : l'.eval (ρ.restrict (vars \ sub_vars) (by aesop)) := by
         rw [h_unfold]
-        rw [←Literal.restrict_correctness l (vars \ sub_vars) ρ]
-        assumption
+        aesop
 
       use l'
 
@@ -216,10 +170,7 @@ lemma Clause.split_correctness {vars} (c : Clause vars)
         Option.some.injEq, and_exists_self] at h_l₁_in_c_in
       obtain ⟨l₂, h_l₂_in_c, h_l₂_vars⟩ := h_l₁_in_c_in
       rw [Clause.eval_eq_false_iff_all_falsified_literals] at h_c
-      specialize h_c l₂ h_l₂_in_c.1
-      rw [←h_l₂_vars]
-      rw [←Literal.restrict_correctness l₂ (vars ∩ sub_vars) ρ]
-      trivial
+      aesop
     · rw [@eval_eq_false_iff_all_falsified_literals]
       intro l₁ h_l₁_in_c_in
       rw [Clause.split] at h_l₁_in_c_in
@@ -228,24 +179,18 @@ lemma Clause.split_correctness {vars} (c : Clause vars)
         Option.some.injEq, and_exists_self] at h_l₁_in_c_in
       obtain ⟨l₂, h_l₂_in_c, h_l₂_vars⟩ := h_l₁_in_c_in
       rw [Clause.eval_eq_false_iff_all_falsified_literals] at h_c
-      specialize h_c l₂ h_l₂_in_c.1
-      rw [←h_l₂_vars]
-      rw [←Literal.restrict_correctness l₂ (vars \ sub_vars) ρ]
-      trivial
+      aesop
 
-
-def CNFFormula.substitute {vars} (φ : CNFFormula vars)
-    {sub_vars : Variables} (ρ : Assignment sub_vars)
-    : CNFFormula (vars \ sub_vars) :=
+def CNFFormula.substitute {vars sub_vars} (φ : CNFFormula vars)
+    (ρ : Assignment sub_vars) : CNFFormula (vars \ sub_vars) :=
   let f := fun c : Clause vars => c.substitute ρ
 
   let φ' := (φ.image f).filterMap id
 
   φ' (by exact fun a a' b a_1 a_2 ↦ Option.eq_of_mem_of_mem a_1 a_2)
 
-lemma CNFFormula.substitute_preimage {vars} (φ : CNFFormula vars)
-    {sub_vars : Variables} (ρ : Assignment sub_vars)
-    : ∀ c ∈ φ.substitute ρ, ∃ c' ∈ φ, c'.substitute ρ = some c := by
-    intro c h_c
-    unfold CNFFormula.substitute at h_c
-    simp_all only [Finset.mem_filterMap, Finset.mem_image, id_eq, exists_eq_right]
+lemma CNFFormula.substitute_preimage {vars sub_vars} {φ : CNFFormula vars}
+    {ρ : Assignment sub_vars} {c} (h_c : c ∈ φ.substitute ρ) :
+    ∃ c' ∈ φ, c'.substitute ρ = some c := by
+  unfold CNFFormula.substitute at h_c
+  simp_all
