BSWLean/Treelike.lean
@@ -22,12 +22,10 @@ class Unsat {vars} (f : CNFFormula vars) : Prop where
   h_unsat : ∀ a, f.eval a = false
 
 @[simp]
-lemma BotClause.variables_is_empty (vars : Variables) : (BotClause vars).variables = ∅ := by
-  aesop
+lemma BotClause.variables_is_empty (vars : Variables) : (BotClause vars).variables = ∅ := by aesop
 
-lemma tree_like_proof_is_correct {vars} {φ : CNFFormula vars} (c : Clause vars)
-    (π : TreeLikeResolution φ c) : ∀ a, φ.eval a → c.eval a := by
-  intro a h_φ_eval_a
+lemma tree_like_proof_is_correct {vars} {φ : CNFFormula vars} {c : Clause vars}
+    (π : TreeLikeResolution φ c) (ρ : Assignment vars) (h_φ_eval_a : φ.eval ρ) : c.eval ρ := by
   rw [CNFFormula.eval_eq_true_iff_all_satisfied_clauses] at h_φ_eval_a
   induction π
   case axiom_clause h_c_in_φ =>
@@ -35,9 +33,8 @@ lemma tree_like_proof_is_correct {vars} {φ : CNFFormula vars} (c : Clause vars)
   case resolve c₁ c₂ v h_v_mem_vars h_v_not_mem_c π₁ π₂ h_resolve ih₁ ih₂ =>
     expose_names
     rw [Clause.eval_eq_true_iff_exists_satisfied_literal]
-    rw [Clause.eval_eq_true_iff_exists_satisfied_literal] at ih₁
-    rw [Clause.eval_eq_true_iff_exists_satisfied_literal] at ih₂
-    by_cases a v h_v_mem_vars
+    rw [Clause.eval_eq_true_iff_exists_satisfied_literal] at ih₁ ih₂
+    by_cases ρ v h_v_mem_vars
     case neg h =>
       obtain ⟨l₁, h_l₁_in_c₁, h_l₁_eval_a⟩ := ih₁
       apply Finset.mem_of_subset h_resolve.left at h_l₁_in_c₁
@@ -45,12 +42,11 @@ lemma tree_like_proof_is_correct {vars} {φ : CNFFormula vars} (c : Clause vars)
       simp only [h_l₁_eval_a, and_true]
       contrapose! h_l₁_in_c₁
       simp only [Finset.union_singleton, Finset.mem_insert, h_l₁_in_c₁, or_false]
-      suffices l₁.eval a ≠ (v.toLiteral h_v_mem_vars).eval a by
+      suffices l₁.eval ρ ≠ (v.toLiteral h_v_mem_vars).eval ρ by
         contrapose! this
         simp only [this]
       rw [h_l₁_eval_a]
-      unfold Literal.eval
-      unfold Variable.toLiteral
+      unfold Literal.eval Variable.toLiteral
       simp only [ne_eq, Bool.true_eq, Bool.not_eq_true]
       exact eq_false_of_ne_true h
     case pos h =>
@@ -60,12 +56,11 @@ lemma tree_like_proof_is_correct {vars} {φ : CNFFormula vars} (c : Clause vars)
       simp only [h_l₂_eval_a, and_true]
       contrapose! h_l₂_in_c₂
       simp only [Finset.union_singleton, Finset.mem_insert, h_l₂_in_c₂, or_false]
-      suffices l₂.eval a ≠ (v.toNegLiteral h_v_mem_vars).eval a by
+      suffices l₂.eval ρ ≠ (v.toNegLiteral h_v_mem_vars).eval ρ by
         contrapose! this
         simp only [this]
       rw [h_l₂_eval_a]
-      unfold Literal.eval
-      unfold Variable.toNegLiteral
+      unfold Literal.eval Variable.toNegLiteral
       simp only [ne_eq, Bool.true_eq, Bool.not_eq_true]
       exact Bool.not_eq_eq_eq_not.mpr h
 
@@ -75,8 +70,7 @@ theorem tree_like_refutation_implies_unsat {vars} {φ : CNFFormula vars}
   unfold TreeLikeRefutation at π
   apply tree_like_proof_is_correct at π
   have : ∀ a : Assignment vars, (BotClause vars).eval a = false := by
-    unfold Clause.eval
-    unfold BotClause
+    unfold Clause.eval BotClause
     exact fun a ↦ rfl
   constructor
   intro a
@@ -85,10 +79,9 @@ theorem tree_like_refutation_implies_unsat {vars} {φ : CNFFormula vars}
   apply π a at h
   contradiction
 
-lemma CNFFormula.substitute_maintains_unsat {vars} (φ : CNFFormula vars)
-    (sub_vars : Variables) (h_subset : sub_vars ⊆ vars) (ρ' : Assignment sub_vars)
-    (h_unsat : Unsat φ)
-  : Unsat (φ.substitute ρ') := by
+lemma CNFFormula.substitute_maintains_unsat {vars sub_vars} {φ : CNFFormula vars}
+    (h_subset : sub_vars ⊆ vars) (ρ' : Assignment sub_vars) (h_unsat : Unsat φ) :
+    Unsat (φ.substitute ρ') := by
   constructor
   intro ρ
   by_contra!
@@ -107,14 +100,11 @@ lemma CNFFormula.substitute_maintains_unsat {vars} (φ : CNFFormula vars)
         )
 
   have h_restrict_in : ρ_full.restrict (sub_vars) (by exact h_subset) = ρ' := by
-    unfold ρ_full
-    unfold Assignment.restrict
-    simp only
-    simp_all only [↓reduceDIte]
+    unfold ρ_full Assignment.restrict
+    simp_all
 
   have h_restrict_out : ρ_full.restrict (vars \ sub_vars) (by exact Finset.sdiff_subset) = ρ := by
-    unfold ρ_full
-    unfold Assignment.restrict
+    unfold ρ_full Assignment.restrict
     simp only
     have : ∀ v ∈ (vars \ sub_vars), v ∉ sub_vars := by
       intro v h_v_mem_vars_sdiff
@@ -123,8 +113,8 @@ lemma CNFFormula.substitute_maintains_unsat {vars} (φ : CNFFormula vars)
     simp_all only [↓reduceDIte]
 
   have h_sub : ∀ c : Clause vars, c.eval ρ_full = true ↔
-    c.substitute ρ' = none ∨
-     ∃ c' : Clause (vars \ sub_vars), c.substitute ρ' = some c' ∧ c'.eval ρ = true := by
+      c.substitute ρ' = none ∨
+      ∃ c' : Clause (vars \ sub_vars), c.substitute ρ' = some c' ∧ c'.eval ρ = true := by
     intro c
     let (c_in, c_out) := c.split sub_vars
     have h' : ρ_full.restrict (vars ∩ sub_vars) (by exact
@@ -135,8 +125,7 @@ lemma CNFFormula.substitute_maintains_unsat {vars} (φ : CNFFormula vars)
       rw [←h_restrict_in]
       simp only [Assignment.double_restrict]
 
-    rw [Clause.split_correctness c sub_vars ρ_full
-    (by exact Finset.inter_subset_left) (by exact Finset.sdiff_subset)]
+    rw [Clause.split_correctness c sub_vars ρ_full]
 
     simp_all only [Bool.or_eq_true]
     constructor
@@ -169,7 +158,7 @@ lemma CNFFormula.substitute_maintains_unsat {vars} (φ : CNFFormula vars)
         obtain ⟨c_out, h_c_out_eval_ρ⟩ := h_exists_c_out
         right
         unfold Clause.substitute at h_c_out_eval_ρ
-        simp_all only [Option.ite_none_left_eq_some, Bool.not_eq_true, Option.some.injEq]
+        simp_all
 
 
   have h_eval_φ : φ.eval ρ_full = true := by
@@ -208,17 +197,17 @@ def TreeLikeResolution.size {vars} {φ : CNFFormula vars} :
   | _, .axiom_clause _ => 1
   | _, .resolve _ _ _ _ _ π₁ π₂ _ => 1 + size π₁ + size π₂
 
-noncomputable def TreeLikeResolution.unsubstitute_rhs {vars} {sub_vars} {c} {φ : CNFFormula vars}
-    (h_subset : sub_vars ⊆ vars) (ρ : Assignment sub_vars)
-    (π : TreeLikeResolution (φ.substitute ρ) c) : Clause vars :=
+noncomputable def TreeLikeResolution.unsubstitute_rhs {vars sub_vars} {c} {φ : CNFFormula vars}
+    {ρ : Assignment sub_vars} (π : TreeLikeResolution (φ.substitute ρ) c)
+    (h_subset : sub_vars ⊆ vars) : Clause vars :=
   match π with
   | .axiom_clause h_c_in_φ =>
     let good := fun c' => (c'.substitute ρ) = some c
-    have : ∃ c' ∈ φ, good c' := by exact CNFFormula.substitute_preimage φ ρ c h_c_in_φ
+    have : ∃ c' ∈ φ, good c' := by exact CNFFormula.substitute_preimage h_c_in_φ
     Classical.choose this
   | .resolve c₁ c₂ x h_x_in h_x_out π₁ π₂ h =>
-    let c₁' := TreeLikeResolution.unsubstitute_rhs h_subset ρ π₁
-    let c₂' := TreeLikeResolution.unsubstitute_rhs h_subset ρ π₂
+    let c₁' := π₁.unsubstitute_rhs h_subset
+    let c₂' := π₂.unsubstitute_rhs h_subset
 
     have h_x_in_vars : x ∈ vars := by
       apply Finset.sdiff_subset
@@ -231,13 +220,13 @@ lemma finset_right_cup {vars} (x : Clause vars) (y : Clause vars) (z : Clause va
     intro h
     exact Finset.union_subset_union h fun ⦃a⦄ a_1 ↦ a_1
 
-lemma TreeLikeResolution.unsubstitute_rhs_variables {vars} {sub_vars} {c} {φ : CNFFormula vars}
-    (h_subset : sub_vars ⊆ vars) (ρ : Assignment sub_vars)
-    (π : TreeLikeResolution (φ.substitute ρ) c) :
-    (TreeLikeResolution.unsubstitute_rhs h_subset ρ π) ⊆
+lemma TreeLikeResolution.unsubstitute_rhs_variables {vars sub_vars} {c} {φ : CNFFormula vars}
+    {ρ : Assignment sub_vars} (π : TreeLikeResolution (φ.substitute ρ) c)
+    (h_subset : sub_vars ⊆ vars) :
+    (π.unsubstitute_rhs h_subset) ⊆
       (Clause.combine c ρ.toClause Finset.sdiff_disjoint).convert_trivial vars (by aesop)
       := by
-  let c' := (TreeLikeResolution.unsubstitute_rhs h_subset ρ π)
+  let c' := π.unsubstitute_rhs h_subset
   let rhs := (Clause.combine c ρ.toClause Finset.sdiff_disjoint).convert_trivial vars (by aesop)
   induction π
   case axiom_clause c h_c_in_φ =>
@@ -245,8 +234,7 @@ lemma TreeLikeResolution.unsubstitute_rhs_variables {vars} {sub_vars} {c} {φ : 
 
     let good := fun cl => cl ∈ φ ∧ (Clause.substitute cl ρ) = some c
     have h_c'_good : good c' := by
-      unfold c'
-      unfold TreeLikeResolution.unsubstitute_rhs
+      unfold c' TreeLikeResolution.unsubstitute_rhs
       simp only
       apply Classical.choose_spec
     have h_sub := h_c'_good.right
@@ -254,8 +242,7 @@ lemma TreeLikeResolution.unsubstitute_rhs_variables {vars} {sub_vars} {c} {φ : 
     have := Clause.substitute_combine c' ρ h_subset h_c'_substitute_isSome
     aesop
   case resolve c c₁ c₂ x h_x_in h_x_out π₁ π₂ h h_π₁ h_π₂ =>
-    unfold unsubstitute_rhs
-    unfold Clause.resolve
+    unfold unsubstitute_rhs Clause.resolve
     simp_all only
     refine Finset.union_subset_iff.mpr ?_
     constructor
@@ -271,8 +258,7 @@ lemma TreeLikeResolution.unsubstitute_rhs_variables {vars} {sub_vars} {c} {φ : 
         apply finset_right_cup
         let h' := h.left
         apply Clause.convert_maintains_subset_insert
-        · unfold Variable.toLiteral
-          unfold Literal.convert
+        · unfold Variable.toLiteral Literal.convert
           unfold Variable.toLiteral at h'
           simp_all only
           suffices q : insert (Literal.pos x h_x_in) c = c ∪ {Literal.pos x h_x_in} by
@@ -291,8 +277,7 @@ lemma TreeLikeResolution.unsubstitute_rhs_variables {vars} {sub_vars} {c} {φ : 
         apply finset_right_cup
         let h' := h.right
         apply Clause.convert_maintains_subset_insert
-        · unfold Variable.toNegLiteral
-          unfold Literal.convert
+        · unfold Variable.toNegLiteral Literal.convert
           unfold Variable.toNegLiteral at h'
           simp_all only
           suffices q : insert (Literal.neg x h_x_in) c = c ∪ {Literal.neg x h_x_in} by
@@ -302,10 +287,9 @@ lemma TreeLikeResolution.unsubstitute_rhs_variables {vars} {sub_vars} {c} {φ : 
 
 
 noncomputable def TreeLikeResolution.unsubstitute {vars} {sub_vars} {c} {φ : CNFFormula vars}
-    (h_subset : sub_vars ⊆ vars) (ρ : Assignment sub_vars)
-    (π : TreeLikeResolution (φ.substitute ρ) c)
-: TreeLikeResolution φ (TreeLikeResolution.unsubstitute_rhs h_subset ρ π) :=
-    let c' := (TreeLikeResolution.unsubstitute_rhs h_subset ρ π)
+    {ρ : Assignment sub_vars} (π : TreeLikeResolution (φ.substitute ρ) c)
+    (h_subset : sub_vars ⊆ vars) : TreeLikeResolution φ (π.unsubstitute_rhs h_subset) :=
+    let c' := π.unsubstitute_rhs h_subset
 
     match h_match : π with
     | .axiom_clause h_c_in_φ =>
@@ -313,18 +297,17 @@ noncomputable def TreeLikeResolution.unsubstitute {vars} {sub_vars} {c} {φ : CN
         let good := fun cl => cl ∈ φ ∧ (Clause.substitute cl ρ) = some c
         suffices q : good c' by
           exact q.left
-        unfold c'
-        unfold TreeLikeResolution.unsubstitute_rhs
+        unfold c' TreeLikeResolution.unsubstitute_rhs
         simp [h_match]
         apply Classical.choose_spec
 
       TreeLikeResolution.axiom_clause (by aesop)
     | .resolve c₁ c₂ x h_x_in h_x_out π₁ π₂ h =>
-      let π₁' := unsubstitute h_subset ρ π₁
-      let π₂' := unsubstitute h_subset ρ π₂
+      let π₁' := π₁.unsubstitute h_subset
+      let π₂' := π₂.unsubstitute h_subset
 
-      let c₁' := unsubstitute_rhs h_subset ρ π₁
-      let c₂' := unsubstitute_rhs h_subset ρ π₂
+      let c₁' := π₁.unsubstitute_rhs h_subset
+      let c₂' := π₂.unsubstitute_rhs h_subset
 
       have h_in : x ∈ vars := by
         have : vars \ sub_vars ⊆ vars := by aesop
@@ -332,50 +315,39 @@ noncomputable def TreeLikeResolution.unsubstitute {vars} {sub_vars} {c} {φ : CN
 
       have h_out : x ∉ c'.variables := by
         unfold c'
-        apply Clause.not_in_variables_subset (unsubstitute_rhs h_subset ρ π)
-          ((Clause.combine c ρ.toClause Finset.sdiff_disjoint).convert_trivial vars (by aesop))
-        · exact unsubstitute_rhs_variables h_subset ρ π
-        · have h_not_in_ρ : x ∉ ρ.toClause.variables := by
-            rw [Assignment.toClause_variables]
-            rw [Finset.mem_sdiff] at h_x_in
-            exact h_x_in.right
-          have : x ∉ (c.combine ρ.toClause Finset.sdiff_disjoint).variables := by
-            apply Clause.combine_not_variables
-            · assumption
-            · assumption
-          rw [←Clause.convert_trivial_keeps_variables]
-          assumption
+        apply Clause.not_in_variables_subset (π.unsubstitute_rhs_variables h_subset)
+        have h_not_in_ρ : x ∉ ρ.toClause.variables := by
+          rw [Assignment.toClause_variables]
+          rw [Finset.mem_sdiff] at h_x_in
+          exact h_x_in.right
+        aesop
 
       have : (c₁' ⊆ c' ∪ { x.toLiteral h_in }) ∧
              (c₂' ⊆ c' ∪ { x.toNegLiteral h_in }) := by
         constructor
-        · unfold c'
-          unfold unsubstitute_rhs
+        · unfold c' unsubstitute_rhs
           simp [h_match]
-          unfold Clause.resolve
-          unfold c₁'
+          unfold c₁' Clause.resolve
           refine Finset.subset_insert_iff.mpr ?_
           exact Finset.subset_union_left
-        · unfold c'
-          unfold unsubstitute_rhs
+        · unfold c' unsubstitute_rhs
           simp [h_match]
-          unfold Clause.resolve
-          unfold c₂'
+          unfold c₂' Clause.resolve
           refine Finset.subset_insert_iff.mpr ?_
           exact Finset.subset_union_right
 
       TreeLikeResolution.resolve c₁' c₂' x h_in (by aesop) π₁' π₂' (by aesop)
 
 
-lemma TreeLikeResolution.unsubstitute_size {vars} {sub_vars} {φ : CNFFormula vars}
-    (h_subset : sub_vars ⊆ vars) (ρ : Assignment sub_vars) (c : Clause (vars \ sub_vars))
-    (π : TreeLikeResolution (φ.substitute ρ) c) : (unsubstitute h_subset ρ π).size ≤ π.size := by
+lemma TreeLikeResolution.unsubstitute_size {vars sub_vars} {φ : CNFFormula vars}
+    {ρ : Assignment sub_vars} {c : Clause (vars \ sub_vars)}
+    (π : TreeLikeResolution (φ.substitute ρ) c) (h_subset : sub_vars ⊆ vars) :
+    (π.unsubstitute h_subset).size ≤ π.size := by
   induction π
   case axiom_clause =>
     aesop
   case resolve =>
-    unfold unsubstitute
-    unfold size
+    unfold unsubstitute size
     linarith
 
 def TreeLikeResolution.convert {vars} {φ : CNFFormula vars} {c : Clause vars}
@@ -398,310 +370,271 @@ lemma left_cancel_one {x y : ℕ} : y ≥ 1 → x ≤ y - 1 → 1 + x ≤ 1 + y 
 
 theorem unsat_implies_tree_like_refutation {vars} {φ : CNFFormula vars}
     (h_unsat : Unsat φ) : ∃ π : TreeLikeRefutation φ, π.size ≤ 2 * 2 ^ vars.card - 1 := by
-    induction vars using Finset.induction_on'
-    case empty =>
-      have h := h_unsat.h_unsat
-      have : (BotClause ∅) ∈ φ := by
-        let a : Assignment ∅ := fun v h_v_mem_vars => by
-          exfalso
-          exact (List.mem_nil_iff v).mp h_v_mem_vars
-        specialize h a
-        rw [CNFFormula.eval_eq_false_iff_exists_falsified_clause] at h
-        obtain ⟨c, h_c_in_φ, h_c_eval_a_false⟩ := h
-        have h_c_eq_bot : c = BotClause ∅ := by
-          unfold BotClause
-          rw [@Finset.eq_empty_iff_forall_notMem]
-          intro l h_l_in_c
-          cases l
-          case pos v h_v_mem_vars =>
-            contradiction
-          case neg v h_v_mem_vars =>
-            contradiction
-        rw [←h_c_eq_bot]
-        exact h_c_in_φ
-      use TreeLikeResolution.axiom_clause this
-      simp only [Finset.card_empty, pow_zero]
-      unfold TreeLikeResolution.size
-      trivial
-
-    case insert v vars' h_v_in_vars h_subset h_v_not_in_vars' ih =>
-      let ρ_true : Assignment {v} := (fun _ => fun _ => True)
-      let φ_true := φ.substitute ρ_true
-      let ρ_false : Assignment {v} := (fun _ => fun _ => False)
-      let φ_false := φ.substitute ρ_false
-
-      have h_vars' : (insert v vars') \ {v} = vars' := by
-        rw [@Finset.sdiff_singleton_eq_erase]
-        rw [Finset.erase_insert h_v_not_in_vars']
-
-      have h_unsat_true : Unsat φ_true := by
-        refine CNFFormula.substitute_maintains_unsat φ {v} ?_ (fun x x_1 ↦ decide True) h_unsat
-        exact Finset.union_subset_left fun ⦃a⦄ a_1 ↦ a_1
-
-      have h_unsat_false : Unsat φ_false := by
-        refine CNFFormula.substitute_maintains_unsat φ {v} ?_ (fun x x_1 ↦ decide False) h_unsat
-        exact Finset.union_subset_left fun ⦃a⦄ a_1 ↦ a_1
-
-      rw [←h_vars'] at ih
-
-      obtain ⟨π_true, h_size_π_true⟩ := ih h_unsat_true
-      obtain ⟨π_false, h_size_π_false⟩ := ih h_unsat_false
-
-      let π_true_lifted := TreeLikeResolution.unsubstitute (by aesop) ρ_true π_true
-      let π_false_lifted := TreeLikeResolution.unsubstitute (by aesop) ρ_false π_false
-
-      let also_vars := insert v vars'
-
-      have h_size_π_true_lifted : π_true_lifted.size ≤ 2^also_vars.card - 1 := by
-        unfold π_true_lifted
-        trans π_true.size
-        · exact
-          TreeLikeResolution.unsubstitute_size
-            (of_eq_true
-              (Eq.trans Finset.singleton_subset_iff._simp_1
-                (Eq.trans Finset.mem_insert._simp_1
-                  (Eq.trans (congr (congrArg Or (eq_self v)) (eq_false h_v_not_in_vars'))
-                    (or_false True)))))
-            ρ_true (BotClause (insert v vars' \ {v})) π_true
-        · trans 2 * 2 ^ (insert v vars' \ {v}).card - 1
-          · assumption
-
-          have : (insert v vars' \ {v}) = vars' := by aesop
-          rw [this]
-          have : also_vars.card = vars'.card + 1 := by aesop
-          rw [this]
-          rw [Nat.pow_add']
-
-      have h_size_π_false_lifted : π_false_lifted.size ≤ 2^also_vars.card - 1 := by
-        unfold π_false_lifted
-        trans π_false.size
-        · exact
-          TreeLikeResolution.unsubstitute_size
-            (of_eq_true
-              (Eq.trans Finset.singleton_subset_iff._simp_1
-                (Eq.trans Finset.mem_insert._simp_1
-                  (Eq.trans (congr (congrArg Or (eq_self v)) (eq_false h_v_not_in_vars'))
-                    (or_false True)))))
-            ρ_false (BotClause (insert v vars' \ {v})) π_false
-        · trans 2 * 2 ^ (insert v vars' \ {v}).card - 1
-          · assumption
-
-          have : (insert v vars' \ {v}) = vars' := by aesop
-          rw [this]
-          have : also_vars.card = vars'.card + 1 := by aesop
-          rw [this]
-          rw [Nat.pow_add']
-
-      let c_true := TreeLikeResolution.unsubstitute_rhs (by aesop) ρ_true π_true
-      let c_false := TreeLikeResolution.unsubstitute_rhs (by aesop) ρ_false π_false
-
-      have h_vars' : vars' = insert v vars' \ {v} := by aesop
-      have h_convert : (Finset.disjUnion (insert v vars' \ {v}) {v} (Finset.sdiff_disjoint)) =
-          also_vars := by grind
-      have : vars' ⊆ also_vars := by exact Finset.subset_insert v vars'
-
-      let v_pos : Clause also_vars := {Variable.toLiteral v (Finset.mem_insert_self v vars')}
-      let v_neg : Clause also_vars := {Variable.toNegLiteral v (Finset.mem_insert_self v vars')}
-
-      have ρ_true_clause : ρ_true.toClause.convert also_vars
-        (by
-          intro l h_l
-          have h_ρ_vars := Assignment.toClause_variables ρ_true
-          have : l.variable ∈ ρ_true.toClause.variables := by
-            exact literal_in_clause_variables l ρ_true.toClause h_l
-          rw [h_ρ_vars] at this
-          have : v ∈ also_vars := by exact Finset.mem_insert_self v vars'
-          grind
-        ) = v_neg := by
-        ext l
-        unfold v_neg
-        simp only [Finset.mem_singleton]
-        constructor
-        · intro hh
-          unfold ρ_true at hh
-          unfold Assignment.toClause at hh
-          unfold Assignment.negVariable at hh
-          unfold Clause.convert at hh
-          unfold Literal.convert at hh
-          simp at hh
-          rw [←hh]
-          rfl
-        · intro tmp
-          rw [tmp]
-          have : ρ_true v (by exact Finset.mem_singleton.mpr rfl) = True := by
-            unfold ρ_true
-            simp
-          unfold Clause.convert
-          simp only [Finset.mem_filterMap, Option.dite_none_right_eq_some, Option.some.injEq,
-            and_exists_self]
-          let l' : Literal {v} := Variable.toNegLiteral v (Finset.mem_singleton.mpr rfl)
-          use l'
-          have : l' ∈ ρ_true.toClause := by
-            rw [Assignment.in_toClause]
-            constructor
-            · unfold Literal.variable
-              unfold l'
-              unfold Variable.toNegLiteral
-              grind
-            · unfold l'
-              unfold Variable.toNegLiteral
-              unfold Literal.eval
-              unfold ρ_true
-              simp
-          use this
-          unfold Literal.convert
-          unfold l'
-          unfold Variable.toNegLiteral
-          simp
-
-      have ρ_false_clause : ρ_false.toClause.convert also_vars
-        (by
-          intro l h_l
-          have h_ρ_vars := Assignment.toClause_variables ρ_false
-          have : l.variable ∈ ρ_false.toClause.variables := by
-            exact literal_in_clause_variables l ρ_false.toClause h_l
-          rw [h_ρ_vars] at this
-          have : v ∈ also_vars := by exact Finset.mem_insert_self v vars'
-          grind
-        ) = v_pos := by
-        ext l
-        unfold v_pos
-        simp only [Finset.mem_singleton]
-        constructor
-        · intro hh
-          unfold ρ_false at hh
-          unfold Assignment.toClause at hh
-          unfold Assignment.negVariable at hh
-          unfold Clause.convert at hh
-          unfold Literal.convert at hh
-          simp at hh
-          rw [←hh]
-          rfl
-        · intro tmp
-          rw [tmp]
-          have : ρ_false v (by exact Finset.mem_singleton.mpr rfl) = false := by
-            unfold ρ_false
-            simp
-          unfold Clause.convert
-          simp only [Finset.mem_filterMap, Option.dite_none_right_eq_some, Option.some.injEq,
-            and_exists_self]
-          let l' : Literal {v} := Variable.toLiteral v (Finset.mem_singleton.mpr rfl)
-          use l'
-          have : l' ∈ ρ_false.toClause := by
-            rw [Assignment.in_toClause]
-            constructor
-            · unfold Literal.variable
-              unfold l'
-              unfold Variable.toLiteral
-              grind
-            · unfold l'
-              unfold Variable.toLiteral
-              unfold Literal.eval
-              unfold ρ_false
-              simp
-          use this
-          unfold Literal.convert
-          unfold l'
-          unfold Variable.toLiteral
-          simp
-
-      have h_c_true : c_true ⊆ v_neg := by
-        unfold c_true
-        let h := TreeLikeResolution.unsubstitute_rhs_variables
-            (by exact Finset.union_subset_left fun ⦃a⦄ a_1 ↦ a_1) ρ_true π_true
-        let mid := ((BotClause (insert v vars' \ {v})).combine ρ_true.toClause
-          Finset.sdiff_disjoint).convert_trivial also_vars h_convert
-        suffices h_combine : mid ⊆ v_neg by
-          trans mid
-          · exact h
-          · assumption
-        unfold mid
+  induction vars using Finset.induction_on'
+  case empty =>
+    have h := h_unsat.h_unsat
+    have : (BotClause ∅) ∈ φ := by
+      let a : Assignment ∅ := fun v h_v_mem_vars => by
+        exfalso
+        exact (List.mem_nil_iff v).mp h_v_mem_vars
+      specialize h a
+      rw [CNFFormula.eval_eq_false_iff_exists_falsified_clause] at h
+      obtain ⟨c, h_c_in_φ, h_c_eval_a_false⟩ := h
+      have h_c_eq_bot : c = BotClause ∅ := by
         unfold BotClause
-        unfold Clause.combine
-        simp [Clause.convert_empty]
-        unfold Clause.convert_trivial
-        rw [Clause.convert_convert]
-        · refine Finset.subset_of_eq ρ_true_clause
-        intro l h_l
-        have : l.variable = v := by
-          unfold ρ_true at h_l
-          unfold Assignment.toClause at h_l
-          unfold Assignment.negVariable at h_l
-          unfold Variable.toNegLiteral at h_l
-          simp only [Finset.mem_singleton, decide_true, ↓reduceIte, Finset.mem_filterMap,
-            Option.dite_none_right_eq_some, Option.some.injEq, and_exists_self,
-            exists_prop_eq] at h_l
-          rw [←h_l]
-          rfl
-        rw [this]
-        exact Finset.mem_insert_self v vars'
+        rw [@Finset.eq_empty_iff_forall_notMem]
+        intro l h_l_in_c
+        cases l
+        case pos v h_v_mem_vars =>
+          contradiction
+        case neg v h_v_mem_vars =>
+          contradiction
+      rw [←h_c_eq_bot]
+      exact h_c_in_φ
+    use TreeLikeResolution.axiom_clause this
+    simp only [Finset.card_empty, pow_zero]
+    unfold TreeLikeResolution.size
+    trivial
 
-      have h_c_false : c_false ⊆ v_pos := by
-        unfold c_false
-        let h := TreeLikeResolution.unsubstitute_rhs_variables
-            (by exact Finset.union_subset_left fun ⦃a⦄ a_1 ↦ a_1) ρ_false π_false
-        let mid := ((BotClause (insert v vars' \ {v})).combine ρ_false.toClause
-          Finset.sdiff_disjoint).convert_trivial also_vars h_convert
-        suffices h_combine : mid ⊆ v_pos by
-          trans mid
-          · exact h
-          · assumption
-        unfold mid
-        unfold BotClause
-        unfold Clause.combine
-        simp [Clause.convert_empty]
-        unfold Clause.convert_trivial
-        rw [Clause.convert_convert]
-        · refine Finset.subset_of_eq ρ_false_clause
-        intro l h_l
-        have : l.variable = v := by
-          unfold ρ_false at h_l
-          unfold Assignment.toClause at h_l
-          unfold Assignment.negVariable at h_l
-          unfold Variable.toNegLiteral at h_l
-          unfold Variable.toLiteral at h_l
-          simp only [Finset.mem_singleton, decide_false, Bool.false_eq_true, ↓reduceIte,
-            Finset.mem_filterMap, Option.dite_none_right_eq_some, Option.some.injEq,
-            and_exists_self, exists_prop_eq] at h_l
-          rw [←h_l]
-          rfl
-        rw [this]
-        exact Finset.mem_insert_self v vars'
+  case insert v vars' h_v_in_vars h_subset h_v_not_in_vars' ih =>
+    let ρ_true : Assignment {v} := (fun _ => fun _ => True)
+    let φ_true := φ.substitute ρ_true
+    let ρ_false : Assignment {v} := (fun _ => fun _ => False)
+    let φ_false := φ.substitute ρ_false
 
-      by_cases c_true = ∅
-      case pos h_true_empty =>
-        unfold c_true at h_true_empty
-        let π' := π_true_lifted.convert ∅ h_true_empty
+    have h_vars' : (insert v vars') \ {v} = vars' := by
+      rw [@Finset.sdiff_singleton_eq_erase]
+      rw [Finset.erase_insert h_v_not_in_vars']
+
+    have h_unsat_true : Unsat φ_true := by
+      refine CNFFormula.substitute_maintains_unsat ?_ ρ_true h_unsat
+      exact Finset.union_subset_left fun ⦃a⦄ a_1 ↦ a_1
+
+    have h_unsat_false : Unsat φ_false := by
+      refine CNFFormula.substitute_maintains_unsat ?_ ρ_false h_unsat
+      exact Finset.union_subset_left fun ⦃a⦄ a_1 ↦ a_1
+
+    rw [←h_vars'] at ih
+
+    obtain ⟨π_true, h_size_π_true⟩ := ih h_unsat_true
+    obtain ⟨π_false, h_size_π_false⟩ := ih h_unsat_false
+
+    let π_true_lifted := π_true.unsubstitute (by aesop)
+    let π_false_lifted := π_false.unsubstitute (by aesop)
+
+    let also_vars := insert v vars'
+
+    have h_size_π_true_lifted : π_true_lifted.size ≤ 2^also_vars.card - 1 := by
+      unfold π_true_lifted
+      trans π_true.size
+      · apply TreeLikeResolution.unsubstitute_size
+      · trans 2 * 2 ^ (insert v vars' \ {v}).card - 1
+        · assumption
+
+        have : (insert v vars' \ {v}) = vars' := by aesop
+        rw [this]
+        have : also_vars.card = vars'.card + 1 := by aesop
+        rw [this]
+        rw [Nat.pow_add']
+
+    have h_size_π_false_lifted : π_false_lifted.size ≤ 2^also_vars.card - 1 := by
+      unfold π_false_lifted
+      trans π_false.size
+      · apply TreeLikeResolution.unsubstitute_size
+      · trans 2 * 2 ^ (insert v vars' \ {v}).card - 1
+        · assumption
+
+        have : (insert v vars' \ {v}) = vars' := by aesop
+        rw [this]
+        have : also_vars.card = vars'.card + 1 := by aesop
+        rw [this]
+        rw [Nat.pow_add']
+
+    let c_true := π_true.unsubstitute_rhs (by aesop)
+    let c_false := π_false.unsubstitute_rhs (by aesop)
+
+    have h_vars' : vars' = insert v vars' \ {v} := by aesop
+    have h_convert : (Finset.disjUnion (insert v vars' \ {v}) {v} (Finset.sdiff_disjoint)) =
+        also_vars := by grind
+    have : vars' ⊆ also_vars := by exact Finset.subset_insert v vars'
+
+    let v_pos : Clause also_vars := {Variable.toLiteral v (Finset.mem_insert_self v vars')}
+    let v_neg : Clause also_vars := {Variable.toNegLiteral v (Finset.mem_insert_self v vars')}
+
+    have ρ_true_clause : ρ_true.toClause.convert also_vars
+      (by
+        intro l h_l
+        have h_ρ_vars := Assignment.toClause_variables ρ_true
+        have : l.variable ∈ ρ_true.toClause.variables := by
+          exact literal_in_clause_variables h_l
+        rw [h_ρ_vars] at this
+        have : v ∈ also_vars := by exact Finset.mem_insert_self v vars'
+        grind
+      ) = v_neg := by
+      ext l
+      unfold v_neg
+      simp only [Finset.mem_singleton]
+      constructor
+      · intro hh
+        unfold ρ_true at hh
+        unfold Assignment.toClause Assignment.negVariable at hh
+        unfold Clause.convert Literal.convert at hh
+        simp at hh
+        rw [←hh]
+        rfl
+      · intro tmp
+        rw [tmp]
+        have : ρ_true v (by exact Finset.mem_singleton.mpr rfl) = True := by
+          unfold ρ_true
+          simp
+        unfold Clause.convert
+        simp only [Finset.mem_filterMap, Option.dite_none_right_eq_some, Option.some.injEq,
+          and_exists_self]
+        let l' : Literal {v} := Variable.toNegLiteral v (Finset.mem_singleton.mpr rfl)
+        use l'
+        have : l' ∈ ρ_true.toClause := by
+          rw [Assignment.in_toClause]
+          constructor
+          · unfold l' Literal.variable Variable.toNegLiteral
+            grind
+          · unfold l' Variable.toNegLiteral Literal.eval ρ_true
+            simp
+        use this
+        unfold l' Literal.convert Variable.toNegLiteral
+        simp
+
+    have ρ_false_clause : ρ_false.toClause.convert also_vars
+      (by
+        intro l h_l
+        have h_ρ_vars := Assignment.toClause_variables ρ_false
+        have : l.variable ∈ ρ_false.toClause.variables := by
+          exact literal_in_clause_variables h_l
+        rw [h_ρ_vars] at this
+        have : v ∈ also_vars := by exact Finset.mem_insert_self v vars'
+        grind
+      ) = v_pos := by
+      ext l
+      unfold v_pos
+      simp only [Finset.mem_singleton]
+      constructor
+      · intro hh
+        unfold ρ_false at hh
+        unfold Assignment.toClause Assignment.negVariable at hh
+        unfold Clause.convert Literal.convert at hh
+        simp at hh
+        rw [←hh]
+        rfl
+      · intro tmp
+        rw [tmp]
+        have : ρ_false v (by exact Finset.mem_singleton.mpr rfl) = false := by
+          unfold ρ_false
+          simp
+        unfold Clause.convert
+        simp only [Finset.mem_filterMap, Option.dite_none_right_eq_some, Option.some.injEq,
+          and_exists_self]
+        let l' : Literal {v} := Variable.toLiteral v (Finset.mem_singleton.mpr rfl)
+        use l'
+        have : l' ∈ ρ_false.toClause := by
+          rw [Assignment.in_toClause]
+          constructor
+          · unfold l' Literal.variable Variable.toLiteral
+            grind
+          · unfold l' Variable.toLiteral Literal.eval ρ_false
+            simp
+        use this
+        unfold l' Literal.convert Variable.toLiteral
+        simp
+
+    have h_c_true : c_true ⊆ v_neg := by
+      unfold c_true
+      let h := π_true.unsubstitute_rhs_variables
+          (by exact Finset.union_subset_left fun ⦃a⦄ a_1 ↦ a_1)
+      let mid := ((BotClause (insert v vars' \ {v})).combine ρ_true.toClause
+        Finset.sdiff_disjoint).convert_trivial also_vars h_convert
+      suffices h_combine : mid ⊆ v_neg by
+        trans mid
+        · exact h
+        · assumption
+      unfold mid BotClause Clause.combine
+      simp [Clause.convert_empty]
+      unfold Clause.convert_trivial
+      rw [Clause.convert_convert]
+      · refine Finset.subset_of_eq ρ_true_clause
+      intro l h_l
+      have : l.variable = v := by
+        unfold ρ_true at h_l
+        unfold Assignment.toClause Assignment.negVariable at h_l
+        unfold Variable.toNegLiteral at h_l
+        simp only [Finset.mem_singleton, decide_true, ↓reduceIte, Finset.mem_filterMap,
+          Option.dite_none_right_eq_some, Option.some.injEq, and_exists_self,
+          exists_prop_eq] at h_l
+        rw [←h_l]
+        rfl
+      rw [this]
+      exact Finset.mem_insert_self v vars'
+
+    have h_c_false : c_false ⊆ v_pos := by
+      unfold c_false
+      let h := π_false.unsubstitute_rhs_variables
+        (by exact Finset.union_subset_left fun ⦃a⦄ a_1 ↦ a_1)
+      let mid := ((BotClause (insert v vars' \ {v})).combine ρ_false.toClause
+        Finset.sdiff_disjoint).convert_trivial also_vars h_convert
+      suffices h_combine : mid ⊆ v_pos by
+        trans mid
+        · exact h
+        · assumption
+      unfold mid BotClause Clause.combine
+      simp [Clause.convert_empty]
+      unfold Clause.convert_trivial
+      rw [Clause.convert_convert]
+      · refine Finset.subset_of_eq ρ_false_clause
+      intro l h_l
+      have : l.variable = v := by
+        unfold ρ_false at h_l
+        unfold Assignment.toClause Assignment.negVariable at h_l
+        unfold Variable.toNegLiteral Variable.toLiteral at h_l
+        simp only [Finset.mem_singleton, decide_false, Bool.false_eq_true, ↓reduceIte,
+          Finset.mem_filterMap, Option.dite_none_right_eq_some, Option.some.injEq,
+          and_exists_self, exists_prop_eq] at h_l
+        rw [←h_l]
+        rfl
+      rw [this]
+      exact Finset.mem_insert_self v vars'
+
+    by_cases c_true = ∅
+    case pos h_true_empty =>
+      unfold c_true at h_true_empty
+      let π' := π_true_lifted.convert ∅ h_true_empty
+      use π'
+      rw [TreeLikeResolution.convert_size]
+      grind
+    case neg h_false_empty =>
+      by_cases c_false = ∅
+      case pos h_empty =>
+        unfold c_false at h_empty
+        let π' := π_false_lifted.convert ∅ h_empty
         use π'
         rw [TreeLikeResolution.convert_size]
         grind
-      case neg h_false_empty =>
-        by_cases c_false = ∅
-        case pos h_empty =>
-          unfold c_false at h_empty
-          let π' := π_false_lifted.convert ∅ h_empty
-          use π'
-          rw [TreeLikeResolution.convert_size]
+      case neg =>
+        have h_c_true : c_true = v_neg := by
+          unfold v_neg
           grind
-        case neg =>
-          have h_c_true : c_true = v_neg := by
-            unfold v_neg
-            grind
-          have h_c_true : c_false = v_pos := by
-            unfold v_pos
-            grind
-          let ξ : TreeLikeResolution φ ∅ := TreeLikeResolution.resolve
-            c_false c_true v (Finset.mem_insert_self v vars')
-            (by exact Disjoint.notMem_of_mem_left_finset (fun ⦃x⦄ a a_1 ↦ a_1) h_v_in_vars)
-            π_false_lifted π_true_lifted (by grind)
-          use ξ
-          unfold TreeLikeResolution.size
-          trans 1 + 2 ^ also_vars.card - 1 + 2 ^ also_vars.card - 1
-          · trans 1 + 2 ^ also_vars.card - 1 + π_true_lifted.size
-            · rw [←right_cancel]
-              apply left_cancel_one
-              · exact Nat.one_le_two_pow
-              · assumption
-            · omega
-          · unfold also_vars
-            omega
+        have h_c_true : c_false = v_pos := by
+          unfold v_pos
+          grind
+        let ξ : TreeLikeResolution φ ∅ := TreeLikeResolution.resolve
+          c_false c_true v (Finset.mem_insert_self v vars')
+          (by exact Disjoint.notMem_of_mem_left_finset (fun ⦃x⦄ a a_1 ↦ a_1) h_v_in_vars)
+          π_false_lifted π_true_lifted (by grind)
+        use ξ
+        unfold TreeLikeResolution.size
+        trans 1 + 2 ^ also_vars.card - 1 + 2 ^ also_vars.card - 1
+        · trans 1 + 2 ^ also_vars.card - 1 + π_true_lifted.size
+          · rw [←right_cancel]
+            apply left_cancel_one
+            · exact Nat.one_le_two_pow
+            · assumption
+          · omega
+        · unfold also_vars
+          omega
