BSWLean.lean
@@ -1,5 +1,5 @@
 import BSWLean.CNF
 import BSWLean.Conversion
-import BSWLean.SuperCNF
 import BSWLean.Substitutions
+import BSWLean.SuperCNF
 import BSWLean.Treelike
